writing to files, taking module as a parameter

src/frontend/Main.fst
@@ -3,18 +3,34 @@ open FStar.All
 open Ast
 open ParserDriver
 module T = Target
-
-#push-options "--warn_error -272"
+open FStar.ST
+#push-options "--warn_error -272" //top-level effects are okay
 let test =
-  let cmdline = FStar.Getopt.cmdline() in
-  match cmdline with
-  | [_; fn] ->
+  let files = Options.parse_cmd_line() in
+  match files with
+  | [fn] ->
     let decls = ParserDriver.parse fn in
     let decls, env = Binding.bind_prog decls in
     let decls = Simplify.simplify_prog env decls in
     // FStar.IO.print_string (String.concat "\n" (List.map Ast.print_decl decls));
     let t_decls = List.map Translate.translate_decl decls in
-    FStar.IO.print_string (Target.print_decls t_decls);
-    FStar.IO.print_string (Target.print_c_entry t_decls)
+
+    let fst_file =
+      FStar.IO.open_write_file
+        (Printf.sprintf "%s/%s.fst"
+          (Options.get_output_dir())
+          (Options.get_module_name())) in
+    FStar.IO.write_string fst_file (Target.print_decls t_decls);
+    FStar.IO.close_write_file fst_file;
+
+    let c_file =
+      FStar.IO.open_write_file
+        (Printf.sprintf "%s/%s_wrapper.c"
+          (Options.get_output_dir())
+          (Options.get_module_name())) in
+    FStar.IO.write_string c_file (Target.print_c_entry t_decls);
+    FStar.IO.close_write_file c_file
+
   | _ ->
+    List.iter (fun x -> FStar.IO.print_string x) files;
     failwith "Not enough arguments"
